src/Lifted.v
@@ -461,5 +461,4 @@ Definition semantics (prog : list expr * list metadata) : semantics :=
                  (step)
                  (initial_state prog)
                  (final_state prog)
-                 (initial_env prog)
-                 (Globalenvs.Genv.to_senv (Globalenvs.Genv.empty_genv unit unit nil)).
+                 (initial_env prog).
